compute a reference matrix for exhaustiveness

Core/Infer/Exhaustiveness.lean
@@ -17,11 +17,11 @@ def lookup_ctor_names (G : GlobalEnv) (T : Ty) : Option ((n : Nat) × Vec String
   | _ => none
 
 -- Given a vector of types, builds a matrix of all possible combination of constructor names
-def enumerate_ctor_names {m : Nat} (G : GlobalEnv) (Ss : Vec Ty m) : Option ((n : Nat) × Fun.Vec (Vec String m) n) := do
+def enumerate_ctor_names {m : Nat} (G : GlobalEnv) (Ss : Vec Ty m) : Option ((n : Nat) × Vec (Vec String m) n) := do
   -- for each type in Ss get all the possible constructors
   let ctors <- (Vec.map (lookup_ctor_names G) Ss).seq
+  return Vec.populate ctors
 
-  sorry
 
 
 namespace Test
@@ -36,29 +36,30 @@ def Γ : GlobalEnv := [
                , ("False", ⟨0, #𝓋[], 0, #𝓋[], gt#"Bool"⟩)]
 ]
 
-#eval Vec.map (lookup_ctor_names Γ) (#𝓋[ (gt#"Maybe" • gt#"Bool"), gt#"Bool"])
-#eval append #𝓋[ "Nothing", "Just"] #𝓋[ "True" , "False" ]
-#eval combine #𝓋[ #𝓋["Nothing", "()"], #𝓋["Just" , "()"]] #𝓋[ "True" , "False" , "Med" ]
-#eval combine #𝓋[ #𝓋[] ] #𝓋["True", "False"]
-#eval combine #𝓋[ #𝓋["Nothing", "()"], #𝓋["Just" , "()"]] #𝓋[ "True" ]
+
+#eval (Vec.map (lookup_ctor_names Γ) (#𝓋[ (gt#"Maybe" • gt#"Bool"), gt#"Bool"])).seq
+#eval enumerate_ctor_names Γ (#𝓋[ (gt#"Maybe" • gt#"Bool"), gt#"Bool", gt#"Bool"])
+#eval Vec.append #𝓋[ "Nothing", "Just"] #𝓋[ "True" , "False" ]
+#eval Vec.combine ⟨2, #𝓋[ #𝓋["Nothing", "()"], #𝓋["Just" , "()"]]⟩ ⟨3 , #𝓋[ "True" , "False" , "Med" ]⟩
+#eval Vec.combine (k := 0) ⟨1, #𝓋[#𝓋[]]⟩ ⟨3 , #𝓋[ "True" , "False" , "Med" ]⟩
 
 end Test
 
 -- returns a matrix of constructor names from a pattern matrix
 @[simp]
-def pattern_to_ctor_tags (ps : Fun.Vec (Pattern m) n) : Fun.Vec (Vec String m) n := λ i =>
+def pattern_to_ctor_names (ps : Fun.Vec (Pattern m) n) : Fun.Vec (Vec String m) n := λ i =>
  Fun.Vec.to (λ j => ((ps i).get_elem j).1)
 
 
 -- Checks that the patterns are exhaustive
-def check_exhaustive (G : GlobalEnv) (Ss : Vec Ty m) (ps : Fun.Vec (Pattern m) n) : Option Unit := do
+def check_exhaustive (G : GlobalEnv) (Ss : Vec Ty m) (ps : Vec (Pattern m) n) : Option Unit := do
   let ⟨_, ref_matrix⟩ <- enumerate_ctor_names G Ss
 
   -- just keep the constructor names from the patterns
-  let ps' := pattern_to_ctor_tags ps
+  let ps' := pattern_to_ctor_names ps.to
 
   -- check that each entry in ref_matrix has an associated entry ps'
-  let mbs := ref_matrix.to.map (λ r => ps'.to.findIdx (λ x => x == r))
+  let mbs := ref_matrix.map (λ r => ps'.to.findIdx (λ x => x == r))
   let _ <- mbs.seq
   return ()
 
